parse, serialize vclist

src/lowparse/LowParse.Spec.VCList.fst
@@ -2,6 +2,7 @@
 
 module LowParse.Spec.VCList
 include LowParse.Spec.Combinators // for seq_slice_append_l
+include LowParse.Spec.Array // for vlarray
 
 module Seq = FStar.Seq
 module U32 = FStar.UInt32
@@ -54,20 +55,22 @@ let synth_inverse_2 (t: Type) (n: nat) : Lemma
   (synth_inverse (synth_nlist_recip #t n) (synth_nlist n))
 = ()
 
-let rec parse_nlist_kind
+let rec parse_nlist_kind'
   (n: nat)
   (k: parser_kind)
-: Tot parser_kind
+: GTot parser_kind
   (decreases n)
 = if n = 0
   then parse_ret_kind
-  else k `and_then_kind` parse_nlist_kind (n - 1) k
+  else k `and_then_kind` parse_nlist_kind' (n - 1) k
+
+#reset-options // enable non-linear arithmetic
 
 let rec parse_nlist_kind_low
   (n: nat)
   (k: parser_kind)
 : Lemma
-  ((parse_nlist_kind n k).parser_kind_low == n `mul` k.parser_kind_low)
+  ((parse_nlist_kind' n k).parser_kind_low == n `mul` k.parser_kind_low)
 = if n = 0
   then ()
   else parse_nlist_kind_low (n - 1) k
@@ -76,7 +79,7 @@ let rec parse_nlist_kind_high
   (n: nat)
   (k: parser_kind)
 : Lemma
-  ((parse_nlist_kind n k).parser_kind_high == (match k.parser_kind_high with
+  ((parse_nlist_kind' n k).parser_kind_high == (match k.parser_kind_high with
     | None -> if n = 0 then Some 0 else None
     | Some b -> Some (n `mul` b)
   ))
@@ -88,7 +91,7 @@ let rec parse_nlist_kind_metadata
   (n: nat)
   (k: parser_kind)
 : Lemma
-  ((parse_nlist_kind n k).parser_kind_metadata == (if n = 0 then Some ParserKindMetadataTotal else k.parser_kind_metadata))
+  ((parse_nlist_kind' n k).parser_kind_metadata == (if n = 0 then Some ParserKindMetadataTotal else k.parser_kind_metadata))
 = if n = 0
   then ()
   else parse_nlist_kind_metadata (n - 1) k
@@ -97,12 +100,33 @@ let rec parse_nlist_kind_subkind
   (n: nat)
   (k: parser_kind)
 : Lemma
-  ((parse_nlist_kind n k).parser_kind_subkind == (
+  ((parse_nlist_kind' n k).parser_kind_subkind == (
     if n = 0 then Some ParserStrong else k.parser_kind_subkind
   ))
 = if n = 0
   then ()
   else parse_nlist_kind_subkind (n - 1) k
+
+inline_for_extraction
+let parse_nlist_kind
+  (n: nat)
+  (k: parser_kind)
+: Tot (k' : parser_kind { k' == parse_nlist_kind' n k })
+= [@inline_let] let _ =
+    parse_nlist_kind_low n k;
+    parse_nlist_kind_high n k;
+    parse_nlist_kind_metadata n k;
+    parse_nlist_kind_subkind n k
+  in
+  {
+    parser_kind_low = n `mul` k.parser_kind_low;
+    parser_kind_high = (match k.parser_kind_high with
+    | None -> if n = 0 then Some 0 else None
+    | Some b -> Some (n `mul` b)
+    );
+    parser_kind_metadata = (if n = 0 then Some ParserKindMetadataTotal else k.parser_kind_metadata);
+    parser_kind_subkind = (if n = 0 then Some ParserStrong else k.parser_kind_subkind);
+  }
 
 let rec parse_nlist'
   (n: nat)
@@ -207,3 +231,202 @@ let serialize_nlist_cons
   ))
 = serialize_synth_eq _ (synth_nlist n) (serialize_nondep_then _ s () _ (serialize_nlist' n s)) (synth_nlist_recip n) () (a :: q);
   serialize_nondep_then_eq _ s () _ (serialize_nlist' n s) (a, q)
+
+(* variable-count lists proper *)
+
+let bounded_count_prop
+  (min max: nat)
+  (x: U32.t)
+: GTot bool
+= min <= U32.v x && U32.v x <= max
+
+inline_for_extraction
+let bounded_count (min max: nat) : Tot Type = (x: U32.t { bounded_count_prop min max x == true } )
+
+inline_for_extraction
+let parse_vclist_payload_kind
+  (min: nat)
+  (max: nat { min <= max } )
+  (k: parser_kind)
+: Tot parser_kind
+= {
+    parser_kind_low = min `mul` k.parser_kind_low;
+    parser_kind_high = (match k.parser_kind_high with
+    | None -> if max = 0 then Some 0 else None
+    | Some b -> Some (max `mul` b)
+    );
+    parser_kind_metadata = (if max = 0 then Some ParserKindMetadataTotal else if min = 0 && k.parser_kind_metadata <> Some ParserKindMetadataTotal then None else k.parser_kind_metadata);
+    parser_kind_subkind = (if max = 0 then Some ParserStrong else if min = 0 && k.parser_kind_subkind <> Some ParserStrong then None else k.parser_kind_subkind);
+  }
+
+#push-options "--z3rlimit 16"
+
+let parse_vclist_payload_kind_is_weaker_than
+  (min: nat)
+  (max: nat)
+  (n: nat { min <= n /\ n <= max })
+  (k: parser_kind)
+: Lemma
+  (parse_vclist_payload_kind min max k `is_weaker_than` parse_nlist_kind n k)
+  [SMTPat (parse_vclist_payload_kind min max k `is_weaker_than` parse_nlist_kind n k)]
+= ()
+
+#pop-options
+
+inline_for_extraction
+let synth_vclist_payload
+  (min: nat)
+  (max: nat)
+  (n: bounded_count min max)
+  (#t: Type)
+  (x: nlist (U32.v n) t)
+: Tot (vlarray t min max)
+= x
+
+let parse_vclist_payload
+  (min: nat)
+  (max: nat)
+  (#k: parser_kind)
+  (#t: Type)
+  (p: parser k t)
+  (n: bounded_count min max)
+: Tot (parser (parse_vclist_payload_kind min max k) (vlarray t min max))
+= weaken (parse_vclist_payload_kind min max k) (parse_synth (parse_nlist (U32.v n) p) (synth_vclist_payload min max n))
+
+inline_for_extraction
+let parse_vclist_kind
+  (min: nat)
+  (max: nat { min <= max } )
+  (lk: parser_kind)
+  (k: parser_kind)
+: Tot parser_kind
+= parse_filter_kind lk `and_then_kind` parse_vclist_payload_kind min max k
+
+inline_for_extraction
+let synth_bounded_count
+  (min: nat)
+  (max: nat { min <= max } )
+  (x: U32.t { bounded_count_prop min max x == true } )
+: Tot (bounded_count min max)
+= x
+
+abstract
+let parse_vclist_and_then_cases_injective
+  (min: nat)
+  (max: nat { min <= max } )
+  (#k: parser_kind)
+  (#t: Type)
+  (p: parser k t)
+: Lemma
+  (and_then_cases_injective (parse_vclist_payload min max p))
+  [SMTPat   (and_then_cases_injective (parse_vclist_payload min max p))]
+=
+    and_then_cases_injective_intro #(bounded_count min max) (parse_vclist_payload min max p) (fun x1 x2 b1 b2 ->
+    parse_synth_eq (parse_nlist (U32.v x1) p) (synth_vclist_payload min max x1) b1;
+    parse_synth_eq (parse_nlist (U32.v x2) p) (synth_vclist_payload min max x2) b2
+  )
+
+abstract
+let parse_vclist
+  (min: nat)
+  (max: nat { min <= max } )
+  (#lk: parser_kind)
+  (lp: parser lk U32.t)
+  (#k: parser_kind)
+  (#t: Type)
+  (p: parser k t)
+: Tot (parser (parse_vclist_kind min max lk k) (vlarray t min max))
+= ((lp `parse_filter` bounded_count_prop min max) `parse_synth` synth_bounded_count min max) `and_then` parse_vclist_payload min max p 
+
+abstract
+let parse_vclist_eq
+  (min: nat)
+  (max: nat { min <= max } )
+  (#lk: parser_kind)
+  (lp: parser lk U32.t)
+  (#k: parser_kind)
+  (#t: Type)
+  (p: parser k t)
+  (b: bytes)
+: Lemma
+  (parse (parse_vclist min max lp p) b == (match parse lp b with
+  | None -> None
+  | Some (n, consumed_n) ->
+    if min <= U32.v n && U32.v n <= max
+    then
+      let b_payload = Seq.slice b consumed_n (Seq.length b) in
+      match parse (parse_nlist (U32.v n) p) b_payload with
+      | None -> None
+      | Some (l, consumed_l) ->
+        Some (l, consumed_n + consumed_l)
+    else None
+  ))
+= and_then_eq ((lp `parse_filter` bounded_count_prop min max) `parse_synth` synth_bounded_count min max) (parse_vclist_payload min max p) b;
+  parse_synth_eq (lp `parse_filter` bounded_count_prop min max) (synth_bounded_count min max) b;
+  parse_filter_eq lp (bounded_count_prop min max) b;
+  match parse lp b with
+  | None -> ()
+  | Some (n, consumed_n) ->
+    if min <= U32.v n && U32.v n <= max
+    then
+      let b_payload = Seq.slice b consumed_n (Seq.length b) in
+      let n : bounded_count min max = n in
+      parse_synth_eq #_ #(nlist (U32.v n) t) #(vlarray t min max) (parse_nlist (U32.v n) p) (synth_vclist_payload min max n) b_payload
+    else ()
+
+let bare_serialize_vclist
+  (min: nat)
+  (max: nat { min <= max /\ max < 4294967296 } )
+  (#lk: parser_kind)
+  (#lp: parser lk U32.t)
+  (ls: serializer lp)
+  (#k: parser_kind)
+  (#t: Type)
+  (#p: parser k t)
+  (s: serializer p { k.parser_kind_subkind == Some ParserStrong } )
+  (l: vlarray t min max)
+: GTot bytes
+= let n = L.length l in
+  let un = U32.uint_to_t n in
+  serialize ls un `Seq.append` serialize (serialize_nlist n s) l
+
+let bare_serialize_vclist_correct
+  (min: nat)
+  (max: nat { min <= max /\ max < 4294967296 } )
+  (#lk: parser_kind)
+  (#lp: parser lk U32.t)
+  (ls: serializer lp  { lk.parser_kind_subkind == Some ParserStrong } )
+  (#k: parser_kind)
+  (#t: Type)
+  (#p: parser k t)
+  (s: serializer p { k.parser_kind_subkind == Some ParserStrong } )
+: Lemma
+  (serializer_correct (parse_vclist min max lp p) (bare_serialize_vclist min max ls s))
+= let prf (x: vlarray t min max)
+  : Lemma
+    (let fx = bare_serialize_vclist min max ls s x in
+      parse (parse_vclist min max lp p) fx == Some (x, Seq.length fx))
+  = let fx = bare_serialize_vclist min max ls s x in
+    parse_vclist_eq min max lp p fx;
+    let n = L.length x in
+    let un = U32.uint_to_t n in
+    let fn = serialize ls un in
+    parse_strong_prefix lp fn fx;
+    let fl = serialize (serialize_nlist n s) x in
+    assert (fl `Seq.equal` Seq.slice fx (Seq.length fn) (Seq.length fx))
+  in
+  Classical.forall_intro prf
+
+let serialize_vclist
+  (min: nat)
+  (max: nat { min <= max /\ max < 4294967296 } )
+  (#lk: parser_kind)
+  (#lp: parser lk U32.t)
+  (ls: serializer lp  { lk.parser_kind_subkind == Some ParserStrong } )
+  (#k: parser_kind)
+  (#t: Type)
+  (#p: parser k t)
+  (s: serializer p { k.parser_kind_subkind == Some ParserStrong } )
+: Tot (serializer (parse_vclist min max lp p))
+= [@inline_let] let _ = bare_serialize_vclist_correct min max ls s in
+  bare_serialize_vclist min max ls s
